Modularize Correctness.NFA

correctness/RegexCorrectness/NFA/Semantics/ProofData/Loop.lean
@@ -1,4 +1,6 @@
-import RegexCorrectness.NFA.Semantics.ProofData.Basic
+module
+
+public import RegexCorrectness.NFA.Semantics.ProofData.Basic
 import RegexCorrectness.NFA.Semantics.ProofData.Compile
 
 set_option autoImplicit false
@@ -16,7 +18,7 @@ it must have looped `nfaExpr` before `n` times, followed by the last step from `
 A `Loop` term corresponds to such a loop. The `last` variant corresponds to the last step,
 and the `loop` variant extracts the first iteration and the remaining loop.
 -/
-inductive Loop {s : String} : Pos s → Pos s → List (Nat × Pos s) → Prop where
+public inductive Loop {s : String} : Pos s → Pos s → List (Nat × Pos s) → Prop where
   | last {pos} (step : nfa'.Step nfa.nodes.size nfa'.start pos next pos .none) : Loop pos pos []
   | loop {pos pos' pos'' update₁ update₂}
     (path : nfa'.Path nfaPlaceholder.nodes.size nfaExpr.start pos nfaPlaceholder.start pos' update₁)
@@ -117,7 +119,7 @@ theorem Loop.introAux {s : String} {pos pos' : Pos s} {i j update}
           exact step.liftBound' gt
         exact ⟨itm, update₁ ::ₒ update₃, update₄, .more step path', loop', by simp [equ]⟩
 
-theorem Loop.intro {s : String} {pos pos' : Pos s} {update}
+public theorem Loop.intro {s : String} {pos pos' : Pos s} {update}
   (wf : nfa.WellFormed) (next_lt : next < nfa.nodes.size)
   (path : nfa'.Path nfa.nodes.size nfa'.start pos next pos' update) :
   Loop pos pos' update := by
